

Beatriz Miranda Bezerra

Teorema do Binômio

① $(1+2x^2)^6 \rightarrow T_{k+1} = \binom{6}{k} \cdot 1^{6-k} \cdot (2x^2)^k$

$T_{k+1} = \binom{6}{k} \cdot (2x^2)^k$

$2k=8$
 $k=8/2$
 $k=4$

$$T_5 = \binom{6}{4} \cdot (2x^2)^4 = \frac{6 \cdot 5}{2} \cdot 16 \cdot x^8 = 15 \cdot 16 \cdot x^8 = \boxed{240 \cdot x^8} \text{ (C)}$$

② $(14x-13y)^{237}$ $x=1$ e $y=1 \rightarrow (14-13)^{237} = 1^{237} = \boxed{1} \text{ (B)}$

③ $(x+a)^n = 1386x^5$

$$T_{k+1} = \binom{n}{k} x^{n-k} \cdot a^k$$

$$T_{k+1} = \binom{11}{k} x^{11-k} a^k$$

$$x^{11-k} = x^5$$
$$11-k=5$$
$$k=6$$

$$T_7 = \binom{11}{6} x^5 a^6 \rightarrow 1386 = \binom{11}{6} a^6 = \frac{11 \cdot 10 \cdot 9 \cdot 8 \cdot 7}{5 \cdot 4 \cdot 3 \cdot 2} a^6$$

$$1386 = 462 a^6 \rightarrow a^6 = \frac{1386}{462} \rightarrow a^6 = 3 \rightarrow \sqrt[6]{a^6} = \sqrt[6]{3}$$

$$\therefore \boxed{a = \sqrt[6]{3}} \text{ (A)}$$

$$\textcircled{4} \left(x + \frac{1}{x^2}\right)^9 = (x + x^{-2})^9$$

$$T_{k+1} = \binom{9}{k} \cdot x^{9-k} \cdot (x^{-2})^k$$

$$9k - 2k = 0$$

$$9 - 3k = 0$$

$$k = 9/3$$

$$k = 3$$

$$T_4 = \binom{9}{3} \cdot x^6 \cdot (x^{-2})^3 = \binom{9}{3} \cdot x^6 \cdot x^{-6} = \binom{9}{3} \quad (D)$$

$$\textcircled{5} \left(x + \frac{1}{x^2}\right)^m = (x + x^{-2})^m \quad T_{k+1} = \binom{m}{k} x^{m-k} (x^{-2})^k$$

$m - k - 2k = m - 3k = 0 \rightarrow k = m/3 \therefore$ Para que $k \in \mathbb{N}$, m deve ser divisível por 3
(c)

$$\textcircled{6} (3x^3 + 2x^{-2})^5 = \binom{5}{0} (3x^3)^5 (2x^{-2})^0 + \binom{5}{1} (3x^3)^4 (2x^{-2})^1 + \binom{5}{2} (3x^3)^3 (2x^{-2})^2 +$$

$$+ \binom{5}{3} (3x^3)^2 (2x^{-2})^3 + \binom{5}{4} (3x^3)^1 (2x^{-2})^4 + \binom{5}{5} (3x^3)^0 (2x^{-2})^5$$

$$243x^{15} + \frac{810}{x^2} + \frac{1080x^9}{x^4} + 720 + \frac{240x^2}{x^8} + \frac{32}{x^{10}}$$

termo independente (e)

7) soma dos coeficientes $(2x+y)^5$ de $x=1$ e $y=1$

$$\rightarrow (2+1)^5 \rightarrow 3^5 = 243 \text{ (c)}$$